hol/p4_from_json/p4_from_jsonScript.sml
@@ -1,0 +1,54 @@
+open HolKernel boolLib liteLib simpLib Parse bossLib;
+
+val _ = new_theory "p4_from_json";
+
+open stringTheory;
+open parse_jsonTheory;
+
+(******************)
+(* PRE-PROCESSING *)
+
+(* NOTE: In the petr4 JSON output, a body can be an array, with Unparsed (a string)
+ * being the first element, and [\"unused\"] (with quotation marks) presumably
+ * being a singleton log message, using \" instead of ", as the second.
+ * *)
+(* Pre-processing will delete duplicate quotation marks and backslashes, leaving
+ * only single quotation marks *)
+Definition p4_preprocess_str:
+(p4_preprocess_str [] = []) /\
+(p4_preprocess_str (h::t) =
+  if ((h = #"\"") \/ ((h = #"\\")))
+  then if ((HD t = #"\"") \/ ((HD t = #"\\")))
+       then (p4_preprocess_str t)
+       else (h::(p4_preprocess_str t))
+  else (h::(p4_preprocess_str t)))
+End
+
+
+(*********)
+(* TESTS *)
+
+(*
+
+val simple_in_stream = TextIO.openIn "simple_input.json";
+
+val simple_input = TextIO.inputAll simple_in_stream;
+
+val simple_input_tm = stringLib.fromMLstring simple_input;
+
+val simple_lex_thm = EVAL ``lex ((^simple_input_tm), [])``;
+
+val simple_parse_thm = EVAL ``json_of_string (^simple_input_tm)``;
+
+
+val vss_in_stream = TextIO.openIn "vss_input.json";
+
+val vss_input = TextIO.inputAll vss_in_stream;
+
+val vss_input_tm = stringLib.fromMLstring vss_input;
+
+val vss_lex_thm = EVAL ``lex (p4_preprocess_str (^vss_input_tm), [])``;
+
+val vss_parse_thm = EVAL ``json_of_string (p4_preprocess_str (^vss_input_tm))``;
+
+*)
